Weidenbach_Book/IsaSAT_Trail.thy
@@ -34,25 +34,27 @@ definition op_map :: "('b \<Rightarrow> 'a::default) \<Rightarrow> 'a \<Rightarr
   \<open>op_map R e xs = do {
     let zs = replicate (length xs) e;
     (_, zs) \<leftarrow> WHILE\<^sub>T\<^bsup>\<lambda>(i,zs). i \<le> length xs \<and> take i zs = map R (take i xs) \<and>
-        length zs = length xs\<^esup>
+        length zs = length xs \<and> (\<forall>k\<ge>i. k < length xs \<longrightarrow> zs ! k = e)\<^esup>
       (\<lambda>(i, zs). i < length zs)
       (\<lambda>(i, zs). do {ASSERT(i < length zs); RETURN (i+1, zs[i := R (xs!i)])})
       (0, zs);
     RETURN zs
      }\<close>
 
+lemma fucck_it: \<open>(\<forall>k\<ge>i. P k) \<Longrightarrow> k\<ge>i \<Longrightarrow> P k\<close>
+  by auto
+
 lemma op_map_map: \<open>op_map R e xs \<le> RETURN (map R xs)\<close>
   unfolding op_map_def Let_def
-  apply (refine_vcg WHILEIT_rule[where R=\<open>measure (\<lambda>(i,_). length xs - i)\<close>])
-  apply (auto simp: hd_conv_nth take_Suc_conv_app_nth list_update_append split: nat.splits)
-  done
+  by (refine_vcg WHILEIT_rule[where R=\<open>measure (\<lambda>(i,_). length xs - i)\<close>])
+    (auto simp: hd_conv_nth take_Suc_conv_app_nth list_update_append split: nat.splits)
 
 lemma op_map_map_rel:
   \<open>(op_map R e, RETURN o (map R)) \<in> \<langle>Id\<rangle>list_rel \<rightarrow>\<^sub>f \<langle>\<langle>Id\<rangle>list_rel\<rangle>nres_rel\<close>
   by (intro frefI nres_relI) (auto simp: op_map_map)
 
-definition arl_option_nat_of_uint32_conv :: \<open>nat option \<Rightarrow> nat option\<close> where
-\<open>arl_option_nat_of_uint32_conv = id\<close>
+definition array_option_nat_of_uint32_conv :: \<open>nat option list \<Rightarrow> nat option list\<close> where
+\<open>array_option_nat_of_uint32_conv = id\<close>
 
 definition array_option_nat_of_uint32 :: "nat option list \<Rightarrow> nat option list nres" where
 \<open>array_option_nat_of_uint32 xs = op_map option_nat_of_uint32_conv None xs\<close>
@@ -64,9 +66,16 @@ sepref_definition array_option_nat_of_uint32_code
   apply (rewrite at \<open>do {let _ = \<hole>; _}\<close> annotate_assn[where A=\<open>array_assn (option_assn nat_assn)\<close>])
   by sepref
 
-thm array_option_nat_of_uint32_code.refine[unfolded array_option_nat_of_uint32_def,
-    FCOMP op_map_map_rel]
+lemma array_option_nat_of_uint32_conv_alt_def:
+  \<open>array_option_nat_of_uint32_conv = map option_nat_of_uint32_conv\<close>
+  unfolding option_nat_of_uint32_conv_def array_option_nat_of_uint32_conv_def by auto
 
+lemma array_option_nat_of_uint32_conv_hnr[sepref_fr_rules]:
+  \<open>(array_option_nat_of_uint32_code, (RETURN \<circ> array_option_nat_of_uint32_conv))
+    \<in> (array_assn (option_assn uint32_nat_assn))\<^sup>k \<rightarrow>\<^sub>a array_assn (option_assn nat_assn)\<close>
+  using array_option_nat_of_uint32_code.refine[unfolded array_option_nat_of_uint32_def,
+    FCOMP op_map_map_rel] unfolding array_option_nat_of_uint32_conv_alt_def
+  by simp
 (* End Move *)
 
 type_synonym tri_bool = \<open>bool option\<close>
@@ -198,6 +207,18 @@ abbreviation trail_pol_fast_assn :: \<open>trail_pol \<Rightarrow> trail_pol_fas
 abbreviation phase_saver_conc where
   \<open>phase_saver_conc \<equiv> array_assn bool_assn\<close>
 
+definition trail_fast_of_slow :: \<open>(nat, nat) ann_lits \<Rightarrow> (nat, nat) ann_lits\<close> where
+  \<open>trail_fast_of_slow = id\<close>
+
+definition trail_pol_fast_of_slow :: \<open>trail_pol \<Rightarrow> trail_pol\<close> where
+  \<open>trail_pol_fast_of_slow =
+    (\<lambda>(M, val, lvls, reason, k). (M, val, lvls, array_option_nat_of_uint32_conv reason, k))\<close>
+
+sepref_definition trail_pol_slow_of_fast_code
+  is \<open>RETURN o trail_pol_fast_of_slow\<close>
+  :: \<open>trail_pol_fast_assn\<^sup>d \<rightarrow>\<^sub>a trail_pol_assn\<close>
+  unfolding trail_pol_fast_of_slow_def
+  by sepref
 
 context isasat_input_ops
 begin
@@ -207,6 +228,18 @@ abbreviation trail_assn :: \<open>(nat, nat) ann_lits \<Rightarrow> trail_pol_as
 
 abbreviation trail_fast_assn :: \<open>(nat, nat) ann_lits \<Rightarrow> trail_pol_fast_assn \<Rightarrow> assn\<close> where
   \<open>trail_fast_assn \<equiv> hr_comp trail_pol_fast_assn trail_pol\<close>
+
+lemma trail_pol_fast_of_slow_trail_fast_of_slow:
+  \<open>(RETURN o trail_pol_fast_of_slow, RETURN o trail_fast_of_slow)
+    \<in> trail_pol \<rightarrow>\<^sub>f \<langle>trail_pol\<rangle> nres_rel\<close>
+  by (intro frefI nres_relI)
+   (auto simp: trail_pol_def trail_pol_fast_of_slow_def array_option_nat_of_uint32_conv_def
+    trail_fast_of_slow_def)
+
+lemma trail_fast_of_slow_hnr[sepref_fr_rules]:
+  \<open>(trail_pol_slow_of_fast_code, RETURN \<circ> trail_fast_of_slow) \<in> trail_fast_assn\<^sup>d \<rightarrow>\<^sub>a trail_assn\<close>
+  using trail_pol_slow_of_fast_code.refine[FCOMP trail_pol_fast_of_slow_trail_fast_of_slow]
+  .
 
 end
 
